ratchet/Denote/Rules.lean
@@ -10,6 +10,7 @@ import Denote.Rules.Regexp
 import Denote.Rules.Cls
 import Denote.Rules.Rescue
 import Denote.Rules.Const
+import Denote.Rules.Bare
 import Denote.Sem.Frame
 
 /-!
